$\omega_{1}^{p}(x)\ и\ \omega_{2}^{q}(x)\ -$ [[Дифференциальная форма|дифференциальные формы]]
$$\omega_{1}^{p}(x) = \sum\limits_{1\leq j_{1}<...<j_{p}\leq n} a_{j_{1}...j_{p}}dx_{j_1}\wedge...\wedge dx_{j_{p}}$$

$$\omega_{2}^{q}(x) = \sum\limits_{1\leq j_{1}<...<j_{q}\leq n} b_{i_{1}...i_{q}}dx_{i_1}\wedge...\wedge dx_{i_{q}}$$

$$\omega_{1}^{p}(x)\wedge\omega_{2}^{q}(x)= \sum\limits_{1\leq j_{1}<...<j_{p}\leq n}\sum\limits_{1\leq j_{1}<...<j_{q}\leq n} a_{j_{1}...j_{p}}b_{i_{1}...i_{q}} dx_{j_1}\wedge...\wedge dx_{j_{p}}\wedge dx_{i_1}\wedge...\wedge dx_{i_{q}}$$
$$\omega_{1}^{p}(x)\wedge\omega_{2}^{q}(x):G\to\Lambda^{p+q}(\Bbb R^{n})$$