
$$
\oint\limits_{\partial D}Pdx+Qdy
=^{?}
\iint\limits_{D}\bigg(\frac{\partial Q}{\partial x} - \frac{\partial P}{\partial y}\bigg)dxdy
$$
Достаточно доказать 
$$
\begin{cases}
\oint\limits_{\partial D}Pdx
=
-\iint\limits_{D}\frac{\partial P}{\partial y}dxdy 
\\
\oint\limits_{\partial D}Qdy
=
\iint\limits_{D}\frac{\partial Q}{\partial x} dxdy
\end{cases}$$
Введем обозначения:
1. График функции $y_{1}(x)-AB$
2. График функции $x_{2}(x)-BC$
3. График функции $y_{2}(x)-CE$
4. График функции $x_1(x)-EA$
$\partial D= ABCEA-$замкнутый контур
Рассмотрим 
$$
\oint\limits_{ABCEA}Pdx
= \underbrace{\int\limits_{AB}P(x,y)dx}_{x=a=const}+\underbrace{\int\limits_{BC}P(x,y)dx}_{x=b=const}+\int\limits_{CE}P(x,y)dx+\int\limits_{EA}P(x,y)dx
=
$$
$$
=
\int\limits_{a}^{b}P(x,y_{1}(x))+0-\int\limits_{a}^{b}P(x,y_{2}(x))dx+0
=
\int\limits_{a}^{b}P(x,y_{1}(x))-\int\limits_{a}^{b}P(x,y_{2}(x))dx
=
$$
$$
=
\int\limits_{a}^{b}\Bigg(\int\limits_{y_{2}(x)}^{y_{1}(x)} \frac{\partial P}{\partial y}(x,y)dy\Bigg)dx
-\int\limits_{a}^{b}dx\int\limits_{y_{1}(x)}^{y_{2}(x)} \frac{\partial P}{\partial y}dy
=
-\iint\limits_{D}\frac{\partial P}{\partial y}dxdy
$$