#Утверждение 
1. $\forall[a,b]\subset(0,+\infty)\implies Г(x)-$ сходится равномерно по $x$ на $[a,b]$
2. $\int\limits_0^{+\infty}(t^{x-1}e^{-t})'_xdt=\int\limits_0^{+\infty}t^{x-1}e^{-t}\ln{t}\ dt$
3. $Г(x+1)=xГ(x)=x!$ 


##### Доказательство $Г(1)=1$
$$Г(1)=\int\limits_0^{+\infty}t^{1-1}e^{-t}\,dt=\int\limits_0^{+\infty}e^{-t}\,dt=-e^{-t}|_0^{+\infty}=-(0-1)=1=0!$$

##### Доказательство $Г(p+1)=pГ(p)$
$$Г(p+1)=\int\limits_0^{+\infty}t^{p+1-1}e^{-t}\,dt=\int\limits_0^{+\infty}t^{p}e^{-t}\,dt=

\begin{vmatrix}
u=t^p & du=p\cdot t^{p-1}dt \\
dv=e^{-t}dt & v=-e^{-t}
\end{vmatrix}=
$$
$$=-t^p\cdot e^{-t}|_0^{+\infty}+p\int\limits_0^{+\infty}t^{p-1}\cdot e^{-t}\,dt=
0+pГ(p)=pГ(p)
$$

##### Доказательство $Г(2)=1$
Т.к. $Г(1)=1$ и $Г(p+1)=pГ(p)$ 
$$Г(2)=1\cdot Г(1)=1\cdot 1 = 1$$
##### Доказательство $Г(n+1)=n!$
$n\in\mathbb{N}:$
$Г(n+1)=nГ(n)$
$Г(3)=2Г(2)=2\cdot1=2!$
$Г(4)=3Г(3)=3\cdot2\cdot1=3!$
Пусть $n=k:\,Г(k+1)=kГ(k)=k!$ верно
$n=k+1:\,Г(k+2)=(k+1)Г(k+1)=(k+1)k!=(k+1)!$

##### Зная, что $Г(p)Г(1-p)=\frac{\pi}{\sin(p\pi)}$ найти $Г(\frac{1}{2})=?$
$$Г(\frac{1}{2})Г(1-\frac{1}{2})=Г(\frac{1}{2})^2=\frac{\pi}{\sin\frac{\pi}{2}}=\pi$$
$$Г(\frac{1}{2})=\sqrt\pi$$